Progress with seq hash interface

theories/coneris/examples/hash/seq_hash_interface.v
@@ -1,146 +1,47 @@
-From clutch.coneris Require Import coneris.
+From clutch.coneris Require Import coneris hash_view_interface.
 
 Set Default Proof Using "Type*".
 
 (** * TODO *)
 (** * For the hash with lock, the lock protects the hash table plus the authoritative part of the maps*)
 
-(* A hash function is collision free if the partial map it
-     implements is an injective function *)
-Definition coll_free (m : gmap nat nat) :=
-  forall k1 k2,
-  is_Some (m !! k1) ->
-  is_Some (m !! k2) ->
-  m !!! k1 = m !!! k2 ->
-  k1 = k2.
+Definition tape_m_elements (tape_m : gmap val (list nat)) :=
+    concat (map_to_list tape_m).*2.
 
-Class hash_view `{!conerisGS Σ} := Hash_View
-{
-  hvG : gFunctors -> Type;
-  hv_name : Type; 
-  hv_auth {L:hvG Σ} : gmap nat nat ->  hv_name -> iProp Σ;
-  hv_frag {L:hvG Σ} : nat -> nat -> hv_name -> iProp Σ;
-
-  hv_auth_timeless {L:hvG Σ} m γ::
-  Timeless (hv_auth (L:=L) m γ);
-  hv_frag_timeless {L:hvG Σ} k v γ::
-  Timeless (hv_frag (L:=L) k v γ);
-  hv_frag_persistent {L:hvG Σ} k v γ::
-  Persistent (hv_frag (L:=L) k v γ);
-  
-  hv_auth_init {L:hvG Σ}:
-  (⊢|==> (∃ γ, hv_auth (L:=L) ∅ γ))%I;
-  hv_auth_coll_free {L:hvG Σ} m γ: hv_auth (L:=L) m γ -∗ ⌜coll_free m⌝;
-  hv_auth_duplicate_frag {L:hvG Σ} m n b γ:
-    m!!n=Some b -> hv_auth (L:=L) m γ ==∗ hv_auth (L:=L) m γ ∗ hv_frag (L:=L) n b γ;
-  hv_auth_frag_agree {L:hvG Σ} m γ k v:
-    hv_auth (L:=L) m γ  ∗ hv_frag (L:=L) k v γ -∗
-    ⌜m!!k=Some v⌝;
-  hv_auth_insert {L:hvG Σ} m n x γ:
-    m!!n=None ->
-    Forall (λ m : nat, x ≠ m) (map (λ p : nat * nat, p.2) (map_to_list m)) ->
-    hv_auth (L:=L) m γ ==∗
-    hv_auth (L:=L) (<[n:=x]> m) γ ∗ hv_frag (L:=L) n x γ             
-}.
-
-Class seq_hash `{!conerisGS Σ} (val_size:nat):= Seq_Hash
+Class seq_hash `{!conerisGS Σ} {h:hash_view} `{!hvG Σ} (val_size:nat):= Seq_Hash
 {
   (** * Operations *)
-  new_counter : val;
+  init_hash : val;
   (* incr_counter : val; *)
   allocate_tape : val;
-  incr_counter_tape : val;
-  read_counter : val;
+  compute_hash : val;
   (** * Ghost state *)
   (** The assumptions about [Σ] *)
-  counterG : gFunctors → Type;
+  seq_hashG : gFunctors → Type;
   (** [name] is used to associate [locked] with [is_lock] *)
   (* tape_name: Type; *)
-  counter_name: Type;
+  seq_hash_tape_gname: Type;
+  
   (** * Predicates *)
-  is_counter {L : counterG Σ} (N:namespace) (counter: val) (γ: counter_name): iProp Σ;
-  (* counter_tapes_auth {L : counterG Σ} (γ: tape_name) (m:gmap loc (list nat)): iProp Σ; *)
-  counter_tapes {L : counterG Σ} (α:val) (ns:list nat): iProp Σ;
-  counter_content_auth {L : counterG Σ} (γ: counter_name) (z:nat): iProp Σ;
-  counter_content_frag {L : counterG Σ} (γ: counter_name) (f:frac) (z:nat): iProp Σ;
+  abstract_seq_hash {L : seq_hashG Σ} (f: val) (m:gmap nat nat) (tape_m : gmap val (list nat)) (γ1:seq_hash_tape_gname) (γ2: hv_name): iProp Σ;
+  concrete_seq_hash {L:seq_hashG Σ} (f:val) (m:gmap nat nat) : iProp Σ; 
+  seq_hash_tape {L : seq_hashG Σ} (α:val) (ns:list nat) (γ: seq_hash_tape_gname) : iProp Σ;
   (** * General properties of the predicates *)
-  #[global] is_counter_persistent {L : counterG Σ} N c γ1 ::
-    Persistent (is_counter (L:=L) N c γ1);
-  (* #[global] counter_tapes_auth_timeless {L : counterG Σ} γ m :: *)
-  (*   Timeless (counter_tapes_auth (L:=L) γ m); *)
-  #[global] counter_tapes_timeless {L : counterG Σ} α ns ::
-    Timeless (counter_tapes (L:=L) α ns);
-  #[global] counter_content_auth_timeless {L : counterG Σ} γ z ::
-    Timeless (counter_content_auth (L:=L) γ z);
-  #[global] counter_content_frag_timeless {L : counterG Σ} γ f z ::
-    Timeless (counter_content_frag (L:=L) γ f z);
-  
-  (* counter_tapes_auth_exclusive {L : counterG Σ} γ m m': *)
-  (* counter_tapes_auth (L:=L) γ m -∗ counter_tapes_auth (L:=L) γ m' -∗ False; *)
-  counter_tapes_exclusive {L : counterG Σ} α ns ns':
-  counter_tapes (L:=L) α ns -∗ counter_tapes (L:=L) α ns' -∗ False;
-  (* counter_tapes_agree {L : counterG Σ} γ α m ns: *)
-  (* counter_tapes_auth (L:=L) γ m -∗ counter_tapes (L:=L) γ α ns -∗ ⌜ m!! α = Some (ns) ⌝; *)
-  counter_tapes_valid {L : counterG Σ} α ns:
-    counter_tapes (L:=L) α ns -∗ ⌜Forall (λ n, n<=3)%nat ns⌝;
-  (* counter_tapes_update {L : counterG Σ} γ α m ns ns': *)
-  (*   Forall (λ x, x<=3%nat) ns'-> *)
-  (*   counter_tapes_auth (L:=L) γ m -∗ counter_tapes (L:=L) γ α ns ==∗ *)
-  (*   counter_tapes_auth (L:=L) γ (<[α := ns']> m) ∗ counter_tapes (L:=L) γ α (ns'); *)
-  counter_tapes_presample {L:counterG Σ} N E γ c α ns ε (ε2 : fin 4%nat -> R):
-  ↑N ⊆ E ->
-  (∀ x, 0<=ε2 x)%R ->
-  (SeriesC (λ n, 1 / 4 * ε2 n)%R <= ε)%R ->
-  is_counter(L:=L) N c γ  -∗
-  counter_tapes (L:=L) α (ns) -∗
-  ↯ ε  -∗
-  state_update E E (∃ n, ↯ (ε2 n) ∗ counter_tapes (L:=L) α (ns ++ [fin_to_nat n]));
+  #[global] abstract_seq_hash_timeless {L : seq_hashG Σ} f m tape_m γ1 γ2 ::
+    Timeless (abstract_seq_hash (L:=L) f m tape_m γ1 γ2);
+  #[global] concrete_seq_hash_timeless {L : seq_hashG Σ} f m ::
+    Timeless (concrete_seq_hash (L:=L) f m);
+  #[global] seq_hash_tape_timeless {L : seq_hashG Σ} α ns γ ::
+    Timeless (seq_hash_tape (L:=L) α ns γ);
 
-  counter_content_auth_exclusive {L : counterG Σ} γ z1 z2:
-    counter_content_auth (L:=L) γ z1 -∗ counter_content_auth (L:=L) γ z2 -∗ False;
-  counter_content_less_than {L : counterG Σ} γ z z' f:
-  counter_content_auth (L:=L) γ z -∗ counter_content_frag (L:=L) γ f z' -∗ ⌜(z'<=z)%nat ⌝;
-  counter_content_frag_combine {L:counterG Σ} γ f f' z z':
-    (counter_content_frag (L:=L) γ f z ∗ counter_content_frag (L:=L) γ f' z')%I ≡
-    counter_content_frag (L:=L) γ (f+f')%Qp (z+z')%nat;
-  counter_content_agree {L : counterG Σ} γ z z':
-    counter_content_auth (L:=L) γ z -∗ counter_content_frag (L:=L) γ 1%Qp z' -∗ ⌜(z'=z)%nat ⌝;
-  counter_content_update {L : counterG Σ} γ f z1 z2 z3:
-    counter_content_auth (L:=L) γ z1 -∗ counter_content_frag (L:=L) γ f z2 ==∗
-    counter_content_auth (L:=L) γ (z1+z3)%nat ∗ counter_content_frag (L:=L) γ f (z2+z3)%nat;
-  
-  (** * Program specs *)
-  new_counter_spec {L : counterG Σ} E N:
-  {{{ True }}} new_counter #() @E
-    {{{ c, RET c; ∃ γ1, is_counter (L:=L) N c γ1 ∗
-                           counter_content_frag (L:=L) γ1 1%Qp 0%nat
-    }}};
-  allocate_tape_spec {L: counterG Σ} N E c γ1 :
-    ↑N ⊆ E->
-    {{{ is_counter (L:=L) N c γ1 }}}
-      allocate_tape #() @ E
-      {{{ (v:val), RET v; counter_tapes (L:=L) v []
-      }}};
-  incr_counter_tape_spec_some {L: counterG Σ} N E c γ1 (Q:nat->iProp Σ) (α:val) n ns:
-    ↑N⊆E ->
-    {{{ is_counter (L:=L) N c γ1 ∗
-        counter_tapes (L:=L) α (n::ns) ∗
-        (  ∀ (z:nat), counter_content_auth (L:=L) γ1 z ={E∖↑N}=∗
-                    counter_content_auth (L:=L) γ1 (z+n) ∗ Q z)
-           
-    }}}
-      incr_counter_tape c α @ E
-                                 {{{ (z:nat), RET (#z, #n); counter_tapes (L:=L) α ns ∗
-                                                          Q z }}}; 
-  read_counter_spec {L: counterG Σ} N E c γ1 Q:
-    ↑N ⊆ E ->
-    {{{  is_counter (L:=L) N c γ1 ∗
-         (∀ (z:nat), counter_content_auth (L:=L) γ1 z ={E∖↑N}=∗
-                    counter_content_auth (L:=L) γ1 z∗ Q z)
-        
-    }}}
-      read_counter c @ E
-      {{{ (n':nat), RET #n'; Q n'
-      }}}
+  seq_hash_presample {L : seq_hashG Σ} f m tape_m γ1 γ2 α E (ε:nonnegreal) ns:
+    abstract_seq_hash (L:=L) f m tape_m γ1 γ2 -∗
+    seq_hash_tape (L:=L) α ns γ1 -∗
+    ↯ (nnreal_div (nnreal_nat (length (map_to_list m) + length (tape_m_elements tape_m))) (nnreal_nat(val_size+1))) -∗
+    ↯ ε -∗
+    state_update E E (∃ (n:nat),
+          ↯ ((nnreal_div (nnreal_nat(val_size+1)) (nnreal_nat (S val_size - (length (map_to_list m) + length (tape_m_elements tape_m))))) *ε) ∗
+          seq_hash_tape (L:=L) α ns γ1 ∗
+          abstract_seq_hash (L:=L) f m tape_m γ1 γ2)
 }.
 
