theories/coneris/examples/hash/hash_view_impl.v
@@ -1,0 +1,118 @@
+From iris.algebra Require Import gset_bij.
+From clutch.coneris Require Export coneris hash_view_interface.
+
+Set Default Proof Using "Type*".
+
+Section hash_view_impl.
+  Context `{Hcon:conerisGS Σ, 
+              HinG: inG Σ (gset_bijR nat nat)}.
+  
+  Definition hash_view_auth m γ := (own γ (gset_bij_auth (DfracOwn 1) (map_to_set pair m)))%I.
+  Definition hash_view_frag k v γ := (own γ (gset_bij_elem k v)).
+
+  Lemma hash_view_auth_coll_free m γ2:
+    hash_view_auth m γ2 -∗ ⌜coll_free m⌝.
+  Proof.
+    rewrite /hash_view_auth.
+    iIntros "H".
+    iDestruct (own_valid with "[$]") as "%H".
+    rewrite gset_bij_auth_valid in H.
+    iPureIntro.
+    intros k1 k2 H1 H2 H3.
+    destruct H1 as [v1 K1].
+    destruct H2 as [v2 H2].
+    assert (v1 = v2) as ->; first by erewrite !lookup_total_correct in H3.
+    unshelve epose proof (H k1 v2 _) as [_ H']; first by rewrite elem_of_map_to_set_pair.
+    unshelve epose proof (H' k2 _) as ->; last done.
+    by rewrite elem_of_map_to_set_pair.
+  Qed.
+
+  Lemma hash_view_auth_duplicate_frag m n b γ2:
+    m!!n=Some b -> hash_view_auth m γ2 ==∗ hash_view_auth m γ2 ∗ hash_view_frag n b γ2.
+  Proof.
+    iIntros (Hsome) "Hauth".
+    rewrite /hash_view_auth/hash_view_frag.
+    rewrite -own_op.
+    iApply own_update; last done.
+    rewrite -core_id_extract; first done.
+    apply bij_view_included.
+    rewrite elem_of_map_to_set.
+    naive_solver.
+  Qed.
+  
+  Lemma hash_view_auth_frag_agree m γ2 k v:
+    hash_view_auth m γ2  ∗ hash_view_frag k v γ2 -∗
+    ⌜m!!k=Some v⌝.
+  Proof.
+    rewrite /hash_view_auth/hash_view_frag.
+    rewrite -own_op.
+    iIntros "H".
+    iDestruct (own_valid with "[$]") as "%H".
+    rewrite bij_both_valid in H.
+    destruct H as [? H].
+    rewrite elem_of_map_to_set in H.
+    iPureIntro.
+    destruct H as (?&?&?&?).
+    by simplify_eq.
+  Qed.
+
+  Lemma hash_view_auth_insert m n x γ:
+    m!!n=None ->
+    Forall (λ m : nat, x ≠ m) (map (λ p : nat * nat, p.2) (map_to_list m)) ->
+    hash_view_auth m γ ==∗
+    hash_view_auth (<[n:=x]> m) γ ∗ hash_view_frag n x γ.
+  Proof.
+    iIntros (H1 H2) "H".
+    rewrite /hash_view_auth/hash_view_frag.
+    rewrite -own_op.
+    iApply own_update; last done.
+    rewrite -core_id_extract; last first.
+    { apply bij_view_included. rewrite elem_of_map_to_set.
+      eexists _, _; split; last done.
+      apply lookup_insert.
+    }
+    etrans; first apply gset_bij_auth_extend; last by rewrite map_to_set_insert_L.
+    - intros b. rewrite elem_of_map_to_set; intros (?&?&?&?).
+      simplify_eq.
+    - intros a. rewrite elem_of_map_to_set; intros (?&?&?&?).
+      simplify_eq.
+      rewrite Forall_map in H2.
+      rewrite Forall_forall in H2.
+      unfold not in H2.
+      eapply H2; [by erewrite elem_of_map_to_list|done].
+  Qed.
+End hash_view_impl.
+
+
+
+Class hvG1 Σ := {hvG1_gsetbijR :: inG Σ (gset_bijR nat nat)}. 
+Program Definition hv_impl `{!conerisGS Σ} : hash_view :=
+  {|
+    hvG := hvG1;
+    hv_name := gname;
+    hv_auth _ m γ := hash_view_auth m γ;
+    hv_frag _ k v γ := hash_view_frag k v γ
+  |}.
+Next Obligation.
+  rewrite /hash_view_auth.
+  iIntros. iApply own_alloc.
+  by rewrite gset_bij_auth_valid.
+Qed.
+Next Obligation.
+  simpl.
+  iIntros.
+  by iApply hash_view_auth_coll_free.
+Qed.
+Next Obligation.
+  simpl. iIntros.
+  by iApply hash_view_auth_duplicate_frag.
+Qed.
+Next Obligation.
+  simpl. iIntros.
+  by iApply hash_view_auth_frag_agree.
+Qed.
+Next Obligation.
+  simpl.
+  iIntros.
+  by iApply hash_view_auth_insert.
+Qed.
