theories/coneris/examples/hash/hash_view_interface.v
@@ -1,0 +1,41 @@
+From clutch.coneris Require Import coneris.
+
+Set Default Proof Using "Type*".
+
+(* A hash function is collision free if the partial map it
+     implements is an injective function *)
+Definition coll_free (m : gmap nat nat) :=
+  forall k1 k2,
+  is_Some (m !! k1) ->
+  is_Some (m !! k2) ->
+  m !!! k1 = m !!! k2 ->
+  k1 = k2.
+
+Class hash_view `{!conerisGS Σ} := Hash_View
+{
+  hvG : gFunctors -> Type;
+  hv_name : Type; 
+  hv_auth {L:hvG Σ} : gmap nat nat ->  hv_name -> iProp Σ;
+  hv_frag {L:hvG Σ} : nat -> nat -> hv_name -> iProp Σ;
+
+  hv_auth_timeless {L:hvG Σ} m γ::
+  Timeless (hv_auth (L:=L) m γ);
+  hv_frag_timeless {L:hvG Σ} k v γ::
+  Timeless (hv_frag (L:=L) k v γ);
+  hv_frag_persistent {L:hvG Σ} k v γ::
+  Persistent (hv_frag (L:=L) k v γ);
+  
+  hv_auth_init {L:hvG Σ}:
+  (⊢|==> (∃ γ, hv_auth (L:=L) ∅ γ))%I;
+  hv_auth_coll_free {L:hvG Σ} m γ: hv_auth (L:=L) m γ -∗ ⌜coll_free m⌝;
+  hv_auth_duplicate_frag {L:hvG Σ} m n b γ:
+    m!!n=Some b -> hv_auth (L:=L) m γ ==∗ hv_auth (L:=L) m γ ∗ hv_frag (L:=L) n b γ;
+  hv_auth_frag_agree {L:hvG Σ} m γ k v:
+    hv_auth (L:=L) m γ  ∗ hv_frag (L:=L) k v γ -∗
+    ⌜m!!k=Some v⌝;
+  hv_auth_insert {L:hvG Σ} m n x γ:
+    m!!n=None ->
+    Forall (λ m : nat, x ≠ m) (map (λ p : nat * nat, p.2) (map_to_list m)) ->
+    hv_auth (L:=L) m γ ==∗
+    hv_auth (L:=L) (<[n:=x]> m) γ ∗ hv_frag (L:=L) n x γ             
+}.
